Refactor source_to_source rewritign into a single function

compiler/backend/source_rewriterScript.sml
@@ -83,145 +83,55 @@ End
 
 (* matching function for expressions *)
 Definition matchesFPexp_def:
-  matchesFPexp p e s =
-    case (p, e) of
-    | Word w1, Lit (Word64 w2) =>
-      if (w1 = w2) then SOME s else NONE
-    | Var n, _ =>
-      (case substLookup s n of
-      | SOME e1 => if e1 = e  then SOME s else NONE
-      | NONE => substUpdate n e s)
-    | Unop op1 p, App (FP_uop op2) [e1] =>
-      (if (op1 = op2)
-      then matchesFPexp p e1 s
-      else NONE)
-    | Binop op1 p1 p2, App (FP_bop op2) [e1;e2] =>
-      (if (op1 = op2)
-      then do
-        s1 <- matchesFPexp p1 e1 s;
-        matchesFPexp p2 e2 s1;
-        od
-      else NONE)
-    | Terop op1 p1 p2 p3, App (FP_top op2) [e1;e2;e3] =>
-      (if (op1 = op2)
-      then do
-        s1 <- matchesFPexp p1 e1 s;
-        s2 <- matchesFPexp p2 e2 s1;
-        matchesFPexp p3 e3 s2;
-        od
-      else NONE)
-  (*
-    | Scope sc1 p, App (FP_sc sc2) [e1] =>
-      (if sc1 = sc2
-      then matchesFPexp p e1 s
-      else NONE) *)
-    | _, _ => NONE
-Termination
-  wf_rel_tac (`measure \ (x,y,z). fp_pat_size x`)
-End
-
-Definition matchesFPexp_comp_def:
-  (matchesFPexp_comp (Word w1) e s =
+  (matchesFPexp (Word w1) e s =
     case e of
     | Lit (Word64 w2) =>
       if (w1 = w2) then SOME s else NONE
     | _ => NONE) /\
-  (matchesFPexp_comp (Var n) e s =
+  (matchesFPexp (Var n) e s =
     case substLookup s n of
     | SOME e1 => if e1 = e  then SOME s else NONE
     | NONE => substUpdate n e s) /\
-  (matchesFPexp_comp (Unop op1 p1) e s =
+  (matchesFPexp (Unop op1 p1) e s =
     case e of
     | App (FP_uop op2) [e1] =>
       (if (op1 = op2)
-      then matchesFPexp_comp p1 e1 s
+      then matchesFPexp p1 e1 s
       else NONE)
     | _ => NONE) /\
-  (matchesFPexp_comp (Binop op1 p1 p2) e s =
+  (matchesFPexp (Binop op1 p1 p2) e s =
     case e of
     | App (FP_bop op2) [e1;e2] =>
       (if (op1 = op2)
        then
-       (case matchesFPexp_comp p1 e1 s of
+       (case matchesFPexp p1 e1 s of
         | NONE => NONE
-        | SOME s1 => matchesFPexp_comp p2 e2 s1)
+        | SOME s1 => matchesFPexp p2 e2 s1)
        else NONE)
     | _ => NONE) /\
-  (matchesFPexp_comp (Terop op1 p1 p2 p3) e s =
+  (matchesFPexp (Terop op1 p1 p2 p3) e s =
    case e of
    | App (FP_top op2) [e1;e2;e3] =>
       (if (op1 = op2)
       then
-       (case matchesFPexp_comp p1 e1 s of
+       (case matchesFPexp p1 e1 s of
         | NONE => NONE
         | SOME s1 =>
-        (case matchesFPexp_comp p2 e2 s1 of
+        (case matchesFPexp p2 e2 s1 of
          | NONE => NONE
-         | SOME s2 => matchesFPexp_comp p3 e3 s2))
+         | SOME s2 => matchesFPexp p3 e3 s2))
        else NONE)
-   | _ => NONE)
-End
-
-Definition matchesFPexp_alt_def:
-  matchesFPexp_alt p e s =
-   (case p of
-   | Word w1 =>
-    (case e of
-    | Lit (Word64 w2) =>
-      if (w1 = w2) then SOME s else NONE
-    | _ => NONE)
-  | Var n =>
-    (case substLookup s n of
-    | SOME e1 => if e1 = e  then SOME s else NONE
-    | NONE => substUpdate n e s)
-  | Unop op1 p1 =>
-    (case e of
-    | App (FP_uop op2) [e1] =>
-      (if (op1 = op2)
-      then matchesFPexp_alt p1 e1 s
-      else NONE)
-    | _ => NONE)
-  | Binop op1 p1 p2 =>
-    (case e of
-    | App (FP_bop op2) [e1;e2] =>
-      (if (op1 = op2)
-       then
-       (case matchesFPexp_alt p1 e1 s of
+      | _ => NONE) ∧
+  (matchesFPexp (Cmp cmp1 p1 p2) e s =
+   case e of
+   | App (FP_cmp cmp2) [e1; e2] =>
+     (if (cmp1 = cmp2) then
+       (case matchesFPexp p1 e1 s of
         | NONE => NONE
-        | SOME s1 => matchesFPexp_alt p2 e2 s1)
+        | SOME s1 => matchesFPexp p2 e2 s1)
        else NONE)
-    | _ => NONE)
-  | Terop op1 p1 p2 p3 =>
-   (case e of
-   | App (FP_top op2) [e1;e2;e3] =>
-      (if (op1 = op2)
-      then
-       (case matchesFPexp_alt p1 e1 s of
-        | NONE => NONE
-        | SOME s1 =>
-        (case matchesFPexp_alt p2 e2 s1 of
-         | NONE => NONE
-         | SOME s2 => matchesFPexp_alt p3 e3 s2))
-       else NONE)
-   | _ => NONE))
-End
-
-Definition matchesFPcexp_def:
-  matchesFPcexp p e s =
-    case p, e of
-    (* | Pred p1 p, App (FP_pred p2) [e1] =>
-      (if (p1 = p2) then matchesFPexp p e1 s else NONE) *)
-    | Cmp cmp1 p1 p2, App (FP_cmp cmp2) [e1; e2] =>
-      (if (cmp1 = cmp2)
-      then do
-        s1 <- matchesFPexp p1 e1 s;
-        matchesFPexp p2 e2 s1;
-        od
-      else NONE)
-    (*
-    | Scope sc1 p, App (FP_sc sc2) [e1] =>
-      (if sc1 = sc2 then matchesFPcexp p e1 s else NONE) *)
-    | _, _ => NONE
+   | _ => NONE) ∧
+  (matchesFPexp (Optimise sc1 p1) e s = NONE)
 End
 
 (* Instantiate a given fp_pattern with a substitution into an expression *)
@@ -242,6 +152,12 @@ Definition appFPexp_def:
       e3 <- appFPexp p3 s;
       return (App (FP_top op) [e1; e2; e3]);
     od) /\
+  appFPexp (Cmp cmp p1 p2) s =
+    (do
+     e1 <- appFPexp p1 s;
+     e2 <- appFPexp p2 s;
+     return (App (FP_cmp cmp) [e1; e2]);
+     od) ∧
   (*
   appFPexp (Scope sc p) s =
     (do
@@ -284,12 +200,7 @@ Definition rewriteFPexp_def:
           (case appFPexp rhs subst of
           | SOME e_opt => rewriteFPexp rwtl e_opt
           | NONE => rewriteFPexp rwtl e)
-      | NONE => case matchesFPcexp lhs e [] of
-          | SOME subst =>
-            (case appFPcexp rhs subst of
-            | SOME e_opt => rewriteFPexp rwtl e_opt
-            | NONE => rewriteFPexp rwtl e)
-          | NONE => rewriteFPexp rwtl e)
+      | NONE => e)
     else e
 End
 
