compiler/backend/proofs/source_rewriterProofsScript.sml
@@ -2,49 +2,24 @@
   Correctness proofs for the expression rewriting function
   Shows that matchesExpr e p = SOME s ==> appExpr p s = SOME e
 *)
-open source_to_sourceTheory fpOptPropsTheory semanticPrimitivesTheory evaluateTheory
-     source_rewriterTheory terminationTheory fpSemPropsTheory;
+open source_rewriterTheory source_to_sourceTheory fpOptTheory fpOptPropsTheory
+     fpSemPropsTheory semanticPrimitivesTheory evaluateTheory
+     semanticsTheory semanticsPropsTheory
+     evaluatePropsTheory terminationTheory fpSemPropsTheory;
 open preamble;
 
 val _ = new_theory "source_rewriterProofs";
-
-Theorem no_match_word_cond:
-  ! w e s1 s2.
-    matchesFPcexp (Word w) e s1 = SOME s2 ==> F
-Proof
-  rpt strip_tac
-  \\ Cases_on `e` \\ fs[matchesFPcexp_def]
-  \\ rename [`App op l`]
-  \\ Cases_on `l` \\ fs[matchesFPcexp_def]
-  \\ Cases_on `t` \\ fs[matchesFPcexp_def]
-QED
-
-Theorem no_match_var_cond:
-  ! n e s1 s2.
-    matchesFPcexp (Var n) e s1 = SOME s2 ==> F
-Proof
-  rpt strip_tac
-  \\ Cases_on `e` \\ fs[matchesFPcexp_def]
-  \\ rename [`App op l`]
-  \\ Cases_on `l` \\ fs[matchesFPcexp_def]
-  \\ Cases_on `t` \\ fs[matchesFPcexp_def]
-QED
 
 Theorem matchExpr_preserving:
   ! p.
     (! e s1 s2.
      matchesFPexp p e s1 = SOME s2 ==>
       substMonotone s1 s2)
-  /\
-    (! ce s1 s2.
-      matchesFPcexp p ce s1 = SOME s2 ==>
-      substMonotone s1 s2)
 Proof
   Induct_on `p`
-  \\ simp[no_match_word_cond, no_match_var_cond]
+  \\ simp[]
   \\ rpt gen_tac \\ TRY conj_tac
   \\ simp[Once matchesFPexp_def, option_case_eq]
-  \\ simp[Once matchesFPcexp_def]
   \\ TRY (fs[substMonotone_def] \\ rpt strip_tac \\ imp_res_tac substLookup_substUpdate \\ rveq \\ fs[] \\ NO_TAC)
   \\ rpt gen_tac
   \\ rpt (TOP_CASE_TAC \\ fs[substMonotone_def]) \\ rpt strip_tac \\ fs[substMonotone_def]
@@ -56,23 +31,19 @@ Theorem appFPexp_weakening:
     (! e s1 s2.
       substMonotone s1 s2 /\
       appFPexp p s1 = SOME e ==>
-      appFPexp p s2 = SOME e) /\
-    (! ce s1 s2.
-      substMonotone s1 s2 /\
-      appFPcexp p s1 = SOME ce ==>
-      appFPcexp p s2 = SOME ce)
+      appFPexp p s2 = SOME e)
 Proof
   Induct_on `p`
   \\ rpt strip_tac \\ fs[]
-  \\ fs[appFPexp_def, appFPcexp_def, pair_case_eq, option_case_eq, substMonotone_def]
+  \\ fs[appFPexp_def, pair_case_eq, option_case_eq, substMonotone_def]
   \\ res_tac \\ fs[]
 QED
 
 val exprSolve_tac =
   (let
-    val thms = CONJ_LIST 2 (SIMP_RULE std_ss [FORALL_AND_THM] appFPexp_weakening)
+    val thm = (SIMP_RULE std_ss [FORALL_AND_THM] appFPexp_weakening)
   in
-  (irule (hd thms) ORELSE irule (hd (tl thms)))
+  (irule thm)
   end)
   \\ asm_exists_tac \\ fs[substMonotone_def]
   \\ rpt strip_tac
@@ -82,15 +53,11 @@ Theorem subst_pat_is_exp:
   ! p.
     (! e s1 s2.
       matchesFPexp p e s1 = SOME s2 ==>
-      appFPexp p s2 = SOME e) /\
-    (! ce s1 s2.
-      matchesFPcexp p ce s1 = SOME s2 ==>
-      appFPcexp p s2 = SOME ce)
+      appFPexp p s2 = SOME e)
 Proof
-  Induct_on `p` \\ rpt gen_tac \\ conj_tac
+  Induct_on `p`
   \\ rpt gen_tac
-  \\ simp[Once matchesFPexp_def]
-  \\ simp[Once matchesFPcexp_def, option_case_eq]
+  \\ simp[Once matchesFPexp_def, option_case_eq]
   \\ rpt (TOP_CASE_TAC \\ fs[]) \\ rpt strip_tac \\ rveq
   \\ fs[Once appFPexp_def, Once appFPcexp_def]
   \\ TRY (imp_res_tac substLookup_substUpdate \\ fs[])
